Parser.v
@@ -195,31 +195,6 @@ Module ParserFn (Import G : Grammar.T).
     constructor; auto.
   Defined.
   
-  Ltac step_h := match goal with
-                 | H : context[match ?x with | _ => _ end] |- _ => destruct x
-                 end.
-  
-  Ltac step_h_eq s := let Heq := fresh s in
-                      match goal with
-                      | H : context[match ?x with | _ => _ end] |- _ =>
-                        destruct x eqn:Heq
-                      end.
-  
-  Ltac step_g := match goal with
-                 | |- context[match ?x with | _ => _ end] => destruct x
-                 end.
-  
-  Ltac step_g_eq s := let Heq := fresh s in
-                      match goal with
-                      | |- context[match ?x with | _ => _ end] => destruct x eqn:Heq
-                      end.
-  
-  Ltac step := simpl in *; (first [step_h | step_g]); auto.
-  Ltac step_eq s := simpl in *; (first [step_h_eq s | step_g_eq s]); auto.
-  Ltac cr := repeat step.
-  Ltac cr_eq s := repeat (step_eq s).
-  Ltac tc := try congruence.
-  
   Open Scope list_scope.
   
   Lemma l_ident_eq_nil :
