Tactics.v
@@ -5,6 +5,31 @@ Open Scope string_scope.
 
 Ltac inv H := inversion H; clear H; subst.
 
+Ltac step_h := match goal with
+               | H : context[match ?x with | _ => _ end] |- _ => destruct x
+               end.
+
+Ltac step_h_eq s := let Heq := fresh s in
+                    match goal with
+                    | H : context[match ?x with | _ => _ end] |- _ =>
+                      destruct x eqn:Heq
+                    end.
+
+Ltac step_g := match goal with
+               | |- context[match ?x with | _ => _ end] => destruct x
+               end.
+
+Ltac step_g_eq s := let Heq := fresh s in
+                    match goal with
+                    | |- context[match ?x with | _ => _ end] => destruct x eqn:Heq
+                    end.
+
+Ltac step := simpl in *; (first [step_h | step_g]); auto.
+Ltac step_eq s := simpl in *; (first [step_h_eq s | step_g_eq s]); auto.
+Ltac cr := repeat step.
+Ltac cr_eq s := repeat (step_eq s).
+Ltac tc := try congruence.
+
 (* Add this to crush *)
 Ltac solveNotFalse := simpl; unfold not; intros; inversion H.
 
